\documentclass[a4paper,11pt]{article}
\usepackage{CJK}
\begin{document}
    \begin{CJK*}{UTF8}{kai}
    QM2 - 将$\psi$代入 \~{F}$\psi = 0$,验证相对论能量动量关系式.
    \end{CJK*}\\[.5cm]
    \begin{CJK*}{UTF8}{song}
    已知
        $$\mbox{\~{F}} = (i\hbar \frac{\partial}{\partial t})^{2} - (-i\hbar \nabla)^{2}c^{2}-m^{2}c^{4}$$
    将
    $\psi = \mathrm{e}^{-i(\overrightarrow{p}\cdot\overrightarrow{x}-Et)/\hbar}$
    代入得
    $$\frac{\partial\psi}{\partial t} = \frac{i\cdot E}{\hbar}\psi \quad,
    \quad \nabla\psi = -\frac{i\cdot p}{\hbar}\psi$$
    $$\frac{\partial ^{2} \psi}{\partial t^{2}} = -\frac{E^{2}}{\hbar ^{2}}\psi \quad,
    \quad \nabla ^{2}\psi = \frac{p^{2}}{\hbar ^{2}}\psi$$
    故由
        $$\mbox{\~{F}}\psi\ =\ (i\hbar)^{2}\cdot (\frac{\partial ^{2} \psi}{\partial t^{2}})
        - (-i\hbar)^{2}\cdot (\nabla ^{2} \psi)
        -m^{2}c^{4}\cdot \psi$$
        $$=(E^{2}-p^{2}c^{2}-m^{2}c^{4})\psi = 0$$
    得
        $$E^{2}=p^{2}c^{2}+m^{2}c^{4}.$$\\
    \begin{CJK*}{UTF8}{kai}
        \begin{flushright}
            \small PB12203077\quad吴奕涛\\
            \footnotesize \today
        \end{flushright}
    \end{CJK*}
    \end{CJK*}
\end{document} 